theories/L/AbstractMachines/TM_LHeapInterpreter/LookupTM.v
@@ -1,7 +1,7 @@
 (** * Heap Lookup *)
 
 From Undecidability Require Import TM.Code.ProgrammingTools LM_heap_def.
-From Undecidability.LAM Require Import TM.Alphabets.
+From Undecidability.L.AbstractMachines.TM_LHeapInterpreter Require Import Alphabets.
 From Undecidability Require Import TM.Code.ListTM TM.Code.CasePair TM.Code.CaseSum TM.Code.CaseNat.
 
 Local Arguments plus : simpl never.
