theories/L/Datatypes/LUnit.v
@@ -5,3 +5,6 @@ From Undecidability.L.Tactics Require Import LTactics GenEncode.
 
 MetaCoq Run (tmGenEncode "unit_enc" unit).
 Hint Resolve unit_enc_correct : Lrewrite.
+
+Lemma size_unit_enc : size(enc tt) = 2. 
+Proof. cbv[enc registered_unit_enc size unit_enc]. lia. Qed. 
