theories/TM/Single/EncodeTapes.v
@@ -41,28 +41,24 @@ Definition isMarked (sig : Type) (s : sigTape sig) : bool :=
   | UnmarkedSymbol _ => false
   end.
 
-(*MOVE*)
 Definition isNilBlank {sig : Type} (s : sigTape sig) : bool :=
   match s with
     NilBlank => true
   | _ => false
   end.
 
-(*MOVE*)
 Definition isLeftBlank {sig : Type} (s : sigTape sig) : bool :=
   match s with
   | LeftBlank _  => true
   | _ => false
   end.
 
-(*MOVE*)
 Definition isRightBlank {sig : Type} (s : sigTape sig) : bool :=
   match s with
   | RightBlank _ => true
   | _ => false
   end.
 
-(*MOVE*)
 Definition isSymbol {sig : Type} (s : sigTape sig) : bool :=
   match s with
   | UnmarkedSymbol _ | MarkedSymbol _ => true
